interpretation of disk ops

BlockCacheSystem/BlockJournalCache.i.dfy
@@ -1,26 +1,32 @@
-include "BlockCache.i.dfy"
+include "BetreeCache.i.dfy"
 include "JournalCache.i.dfy"
 include "BlockJournalDisk.i.dfy"
 
 module BlockJournalCache {
-  import BlockCache
+  import BetreeCache
   import JournalCache
   import D = BlockJournalDisk
   import opened ViewOp
   import UI
 
   datatype Constants = Constants(
-    bc: BlockCache.Constants,
+    bc: BetreeCache.Constants,
     jc: JournalCache.Constants)
 
   datatype Variables = Variables(
-    bc: BlockCache.Variables,
+    bc: BetreeCache.Variables,
     jc: JournalCache.Variables)
+
+  predicate Init(k: Constants, s: Variables)
+  {
+    && BetreeCache.Init(k.bc, s.bc)
+    && JournalCache.Init(k.jc, s.jc)
+  }
 
   predicate NextStep(k: Constants, s: Variables, s': Variables, uiop: UI.Op, dop: D.DiskOp, vop: VOp)
   {
     && VOpAgreesUIOp(vop, uiop)
-    && BlockCache.Next(k.bc, s.bc, s'.bc, dop.bdop, vop)
+    && BetreeCache.Next(k.bc, s.bc, s'.bc, dop.bdop, vop)
     && JournalCache.Next(k.jc, s.jc, s'.jc, dop.jdop, vop)
   }
 
